Challenge/Modexp/Submission/Proofs/Fast/Paths/P11.lean
@@ -37,7 +37,7 @@ def blk1569 :
    opAt 1024 (.Dup ⟨2, by decide⟩),
    opAt 1025 (.Dup ⟨1, by decide⟩),
    opAt 1026 .GT,
-   pushAt 1027 2 1237,
+   pushAt 1027 2 1238,
    opAt 1028 .JUMPI]
 
 /-- Instructions 1672..1726, pc 2595..2346. -/
@@ -46,7 +46,7 @@ def blk1595 :
   [opAt 1029 .POP,
    opAt 1030 .POP,
    opAt 1031 .POP,
-   pushAt 1032 2 4330,
+   pushAt 1032 2 4325,
    opAt 1033 .JUMP]
 
 /-- Instructions 1600..1753, pc 2347..2379. -/
